BISHOP.dfy
@@ -45,6 +45,14 @@ lemma Enclosed_Enclosed(part : Object, whole : Object)
    }
 
 
+lemma HappyFamilies0(next : Object, whole : Object)
+  requires next.Ready()
+   ensures (allInside(next.AMFO, whole) + allOutside(next.AMFO, whole) + allOffside(next.AMFO, whole)) == next.AMFO
+   ensures (allInside({next}, whole) + allOutside({next}, whole) + allOffside({next}, whole)) == {next}
+{
+
+}
+
 
 lemma HappyFamilies(soup : set<Object>, whole : Object, ins: set<Object>, outs: set<Object>, sides: set<Object>)
   requires ins   == allInside(soup, whole)
